Port to work with metacoq-1.0

extraction/plugin/src/mCProd.mli
@@ -1,0 +1,5 @@
+open Datatypes
+
+val on_snd : ('a2 -> 'a3) -> ('a1 * 'a2) -> 'a1 * 'a3
+
+val test_snd : ('a2 -> bool) -> ('a1 * 'a2) -> bool
